Test.Coordinates.fst
@@ -6,15 +6,28 @@ type azType = (az: float{az |-> (~._180 <.|> _180)})
 type psk : eqtype =
   {
     az: azType;
-    um: (um: float{um.(~._90, _90)})
+    um: (um: float{um.(~._90, _90)});
   }
-type cart : eqtype = { x: float; y: float; z: float}
+type cart' : eqtype = { x: float; y: float; z: float }
+let radius (coord: cart') = hypot3 coord.x coord.y coord.z
+type cart = coord: cart'{radius coord = _1}
 
-let psk2cart (coord: psk) = 
+
+let psk2cart (coord: psk) : cart = 
   let x = cos coord.az *. cos coord.um in
   let y = sin coord.az *. cos coord.um in
   let z = sin coord.um in
-  { x = x; y = y; z = z }
+  let coord' = { x = x; y = y; z = z } in
+  
+  let _1_gt_0 () : Lemma (_1 >. _0) = () in
+  simplification_sqr_cos_sin coord.az (cos coord.um);
+  lemma_osn_trig_todj coord.um;
+  assert (sqr x +. sqr y +. sqr z = _1);
+  _1_gt_0 ();
+  _1 `is_sqrt` _1;
+  assert (radius coord' = _1);
+
+  coord'
 
 private let wrap (a: float) : Pure float (requires a.[~._180, _180]) 
   (ensures fun b -> b |-> (~._180 <.|> _180) /\ (a |-> (~._180 <.|> _180) ==> a = b))
@@ -25,8 +38,8 @@ private let wrap (a: float) : Pure float (requires a.[~._180, _180])
 
 let cart2psk (coord: cart) =
   let az = arctg coord.x coord.y in
-  let um = arctg (hypot coord.x coord.y) coord.z in
-  lemma_arctg_x_pos (hypot coord.x coord.y) coord.z;
+  let um = arctg (hypot2 coord.x coord.y) coord.z in
+  lemma_arctg_x_pos (hypot2 coord.x coord.y) coord.z;
   assert (um.(~._90, _90));
   
   let az' = wrap az in
@@ -39,31 +52,6 @@ let lemma_psk2cart (p: psk) : Lemma (cart2psk (psk2cart p) = p) [SMTPat (psk2car
     assert (~._90 >=. ~._180);
     point_inj x (~._90 <|> _90) (~._180 <.|.> _180)
   in
-  let lemma_hypot_cos (h az um: float) : Lemma
-    (requires h = hypot (cos az *. cos um) (sin az *. cos um) /\ um.(~._90, _90))
-    (ensures h = cos um)
-    =
-    let cos_az = cos az in
-    let sin_az = sin az in
-    let cos_um = cos um in
-    lemma_cos_pos um;
-
-    assert (h *. h = (cos_az *. cos_um) *. (cos_az *. cos_um) +. (sin_az *. cos_um) *. (sin_az *. cos_um));
-    assert (h *. h = (cos_az *. cos_um) *. (cos_um *. cos_az) +. (sin_az *. cos_um) *. (cos_um *. sin_az));
-    assoc_mul_right (cos_az *. cos_um) cos_um cos_az;
-    commut_tri_mul cos_az cos_um cos_um;
-    assoc_mul_right (cos_um *. cos_um) cos_az cos_az;
-
-    assoc_mul_right (sin_az *. cos_um) cos_um sin_az;
-    commut_tri_mul sin_az cos_um cos_um;
-    assoc_mul_right (cos_um *. cos_um) sin_az sin_az;
-    assert (h *. h = (cos_um *. cos_um) *. (cos_az *. cos_az) +. (cos_um *. cos_um) *. (sin_az *. sin_az));
-    distrib_add (cos_um *. cos_um) (cos_az *. cos_az) (sin_az *. sin_az);
-    lemma_osn_trig_todj az;
-    mul_one (cos_um *. cos_um);
-    assert (h *. h = cos_um *. cos_um);
-    lemma_hypot_pos h cos_um
-  in
   let lemma_one () : Lemma (_1 <> _0) = ()
   in
   let c = psk2cart p in
@@ -73,9 +61,12 @@ let lemma_psk2cart (p: psk) : Lemma (cart2psk (psk2cart p) = p) [SMTPat (psk2car
   lemma_arctg p.az (cos p.um);
   assert (p'.az = p.az);
 
-  let h = hypot c.x c.y in
-  lemma_hypot_cos h p.az p.um;
-
+  let h = hypot2 c.x c.y in
+  simplification_sqr_cos_sin p.az (cos p.um);
+  assert (h = sqrt (sqr (cos p.um)));
+  lemma_cos_pos p.um;
+  sqr_eq h (cos p.um);
+  assert (h = cos p.um);
   mul_one (cos p.um);
   mul_one (sin p.um);
   assert (p'.um = arctg (cos p.um) (sin p.um));
