Test.Float.Trigonometry.fsti
@@ -11,7 +11,16 @@ val _90  : (x: float{x = of_int 90})
 val sin : float -> (r: float{r.[~._1, _1]})
 val cos : float -> (r: float{r.[~._1, _1]})
 val arctg (x y: float) : (r: float{r.[~._180, _180]})
-val hypot (x y: float) : (r: float{r *. r = x *. x +. y *. y /\ r >=. _0})
+val hypot2 (x y: float) : Pure float (requires True) (ensures fun h ->
+  sqr_gt_0 x; sqr_gt_0 y;
+  distrib_gte_0 (sqr x) (sqr y);
+  (sqr x +. sqr y) >=. _0 /\ h = sqrt (sqr x +. sqr y))
+val hypot3 (x y z: float) : Pure float (requires True) (ensures fun h ->
+  sqr_gt_0 x; sqr_gt_0 y; sqr_gt_0 z;
+  distrib_gte_0 (sqr x) (sqr y);
+  distrib_gte_0 (sqr x +. sqr y) (sqr z);
+  (sqr x +. sqr y +. sqr z) >=. _0 /\ h = sqrt (sqr x +. sqr y +. sqr z))
+
 
 val lemma_sin_odd  (a: float) : Lemma (sin a = ~.(sin ~.a))
 val lemma_cos_even (a: float) : Lemma (cos a = cos ~.a)
@@ -25,8 +34,7 @@ val lemma_sin_90 (a: float{a = of_int 90}) : Lemma (sin a = _1)
 val lemma_cos_90 (a: float{a = of_int 90}) : Lemma (cos a = _0)
 let lemma_sin_cos_90 (a: float{a = of_int 90}) : Lemma (sin a = _1 /\ cos a = _0) = lemma_sin_90 a; lemma_cos_90 a
 
-val lemma_osn_trig_todj (a: float) : Lemma ((sin a *. sin a) +. (cos a *. cos a) = _1 /\
-                                            (cos a *. cos a) +. (sin a *. sin a) = _1)
+val lemma_osn_trig_todj (a: float) : Lemma (sqr (sin a) +. sqr (cos a) = _1)
 
 val lemma_cos_add (a b: float) : Lemma (cos (a +. b) = cos a *. cos b -. sin a *. sin b)
 val lemma_sin_add (a b: float) : Lemma (sin (a +. b) = sin a *. cos b +. cos a *. sin b)
@@ -35,12 +43,18 @@ val lemma_arctg (a: float{a.[~._180, _180]}) (b: not_0) : Lemma (arctg (cos a *.
 
 val lemma_cos_pos (a: float{a.(~._90, _90)}) : Lemma (cos a >. _0)
 
-let lemma_hypot_pos (h: float) (pos: float{pos >=. _0}) : Lemma 
-  (requires h *. h = pos *. pos /\ h >=. _0)
-  (ensures h = pos)
-  =
-  sqr_eq h pos;
-  lte_neg pos _0;
-  match pos >. _0 with
-  | true -> assert (h = ~.pos ==> pos <=. _0)
-  | false -> assert (pos =. _0)
+let simplification_sqr_cos_sin a b : Lemma (sqr (b *. cos a) +. sqr (b *. sin a) = sqr b) =
+  let cos = cos a in
+  let sin = sin a in
+  let bb = sqr (b *. cos) +. sqr (b *. sin) in
+
+  assoc_mul_right (b *. cos) b cos;
+  commut_tri_mul b cos b;
+  assoc_mul_right (b *. b) cos cos;
+  assoc_mul_right (b *. sin) b sin;
+  commut_tri_mul b sin b;
+  assoc_mul_right (b *. b) sin sin;
+  assert (bb = (b *. b) *. (cos *. cos) +. (b *. b) *. (sin *. sin));
+  distrib_add (sqr b) (sqr cos) (sqr sin);
+  lemma_osn_trig_todj a;
+  mul_one (sqr b)
